The Gamma function is a generalization of the factorial function to non-integer values:$$\Gamma(s)=\int_0^\infty t^{s-1}e^{-t}dt,\quad\Re s>0$$The integral converges to a function holomorphic on $\Re s>0$.
**Proof**: let $F_\varepsilon(s)=\int_\varepsilon^{1/\varepsilon}t^{s-1}e^{-t}dt$ which is holomorphic for any $\Re s>0$ ([[Holomorphic Function]])m then it can be estimated that $|\Gamma(s)-F_\varepsilon(s)|\to0$ uniformly, hence $\Gamma$ is holomorphic.
- **Recursion formula**: $\Gamma(s+1)=s\Gamma(s)$ due to integration by parts. [[Lebesgue Integral]]
	- **Extension of factorial**: since $\Gamma(1)=1$ we have that $\Gamma(n)=(n-1)!,\forall n\in\mathbb Z_{\ge1}$.
- **Analytic continuation to $\Im z\le0$**: the function $\Gamma(s),\Re s>0$ can be continued analytically to a meromorphic function on $\mathbb C$ whose singularities are simple poles at $-\mathbb N$, with $$\Res(\Gamma,-n)=\frac{(-1)^n}{n!},\forall n\in\mathbb N$$**Proof**: we continue $\Gamma$ strip by strip. For $\Re s>-1$ let $F_1(s)=\frac{\Gamma(s+1)}{s}$, then since $\Gamma(1)=1$ we know that $F_1$ indeed has a simple pole at $0$ with $\Res(F_1,0)=1$. By [[Analytic Continuation]] we know that $F_1$ is a continuation for $\Gamma$. Repeat this for $\Re s>-m,m\in\mathbb N$ in the following way: $$F_m(s)=\frac{\Gamma(s+m)}{(s+m-1)(s+m-2)\cdots s}$$then $F_m$ is meromorphic in $\Re s>-m$ and has simple poles at $s=0,\cdots,-m+1$ with $$\Res(F_m,-n)=\frac{\Gamma(-n+m)}{(m-1-n)!(-1)(-2)\cdots(-n)}=\frac{(-1)^n}{n!}$$Let $m\to\infty$, and we get a continuation of $\Gamma$ has the stated properties.
	- **Proof via Taylor expansion**: notice that $$\Gamma(s)=\left(\int_0^1+\int_1^\infty\right)t^{s-1}e^{-t}dt=\sum_{n\in\mathbb N}\frac{(-1)^n}{n!(n+s)}+\int_1^\infty t^{s-1}e^{-t}dt$$The second integral is entire, while the summation defines a meromorphic function with poles at $-\mathbb N$, with the correct order and residual. 
	- **Recursion formula for poles**: notice that $\Res(\Gamma(s+1),n)=n\Res(\Gamma(s),n),\forall n\in-\mathbb N$.
- **Euler's reflection formula**: we have $$\Gamma(s)\Gamma(1-s)=\frac{\pi}{\sin\pi s},\quad\forall s\in\mathbb C$$**Proof**: using contour integration we have $$\int_0^\infty\frac{v^{a-1}}{1+v}dv=\int_{-\infty}^\infty\frac{e^{ax}}{1+e^x}dx=\frac{\pi}{\sin\pi a}$$On the other hand, $\Gamma(1-s)=\int_0^\infty e^{-u}u^{-s}du=t\int_0^\infty e^{-vt}(vt)^{-s}dv$ by change of variable $u=vt$. Putting this into $\Gamma(s)\Gamma(1-s)$ and changing the order of integration yields the result.
	- $1/\Gamma(s)=\Gamma(1-s)\frac{\sin\pi s}{\pi}$, hence the simple poles at $\mathbb N\backslash\set{0}$ are canceled by simple zeros of $\sin\pi s$. Therefore $1/\Gamma$ is entire with simple zeros at $-\mathbb N$.
- **Order of $1/\Gamma$**: notice that $\int_1^\infty e^{-t}t^{\sigma}dt\le n!\le n^n\le\exp((\sigma+1)\ln(\sigma+1))$, denoting $\sigma=\Re s$ then $$\begin{align}\left|\frac{1}{\Gamma(s)}\right|&\le\left|\left(\sum_{n\in\mathbb N}\frac{(-1)^n}{n!(n+1-s)}\right)\frac{\sin \pi s}{\pi}\right|+\left|\left(\int_1^\infty e^{-t}t^{-s}dt\right)\frac{\sin \pi s}{\pi}\right|\\&\le C_1+C_2\exp((|\sigma|+1)\ln(|\sigma|+1))\cdot e^{\pi|s|}\\&\le C\exp(C'|s|\ln|s|)\end{align}$$This shows that $\rho(1/\Gamma)=1$.
- **Hadamard factorization for $1/\Gamma$**: we have $$\frac{1}{\Gamma(s)}=e^{\gamma s}s\prod_{n=1}^\infty\left(1+\frac{s}{n}\right)e^{-s/n}$$where $\gamma$ is the Euler constant. [[Special Constant Gallery]]
  **Proof**: by $\rho(1/\Gamma)=1$ assume that $1/\Gamma(s)=e^{As+B}s\prod_{n=1}^\infty\left(1+\frac{s}{n}\right)e^{-s/n}$. By $s\Gamma(s)\to1,s\to0$ we know that $B=0$ while by $\Gamma(1)=1$ we know that $e^{-A}=\prod_{n=1}^\infty(1+1/n)e^{-1/n}=e^{-\gamma}$, therefore $A=\gamma$.
	- **Essential characterization**: the Hadamard factorization shows that Gamma function is characterized by two properties: $\rho(1/\gamma)\le1$, and $1/\Gamma$ has simple poles at $-\mathbb N$ while vanishes nowhere else.
- **logarithmic convexity**: Gamma function is satisfies:
	- A function $f$ is logarithmically convex if $\log\circ f$ is convex.
	- A equivalent expression is $\Gamma''(x)\Gamma(x)>\Gamma'(x)^2$.
- **Stirling's formula**: for $x\to\infty$, we have $\Gamma(x+1)\sim\sqrt{2\pi x}(\frac{x}{e})^x$. [[Series]]
- **Application**
	- For any real number $a,b$, we have $$\int_0^\infty t^be^{-at}dt=\frac{\Gamma(b+1)}{a^{b+1}}$$According to Euler's formula $e^{ix}=\cos x+i\sin x$, integrals involving $\sin x^\alpha,\cos x^\alpha$ can be solved.
	- Used in probability and statistics. [[Distribution Function Gallery]]
	- **$n$-ball with radius $R$**: using [[Integral Calculus on Euclidean Space]] we have $$V_n(R)=\frac{\pi^{n/2}}{\Gamma(\frac{n}{2}+1)}R^n=\alpha(n)R^n,\quad n\in\mathbb N$$where $\alpha(n)=V_n(1)$. By differentiation we get the surface area of $n$-ball as $$S_{n-1}(R)=\frac{n}{R}V_n(R)=\frac{2\pi^{n/2}}{\Gamma(\frac{n}{2})}R^{n-1}=n\alpha(n)R^{n-1}$$
## Beta function
The beta function, also called the Euler integral of the first kind, is defined by $$B(z_1,z_2)=\int_0^1t^{z_1-1}(1-t)^{z_2-1}dt,\qquad\Re(z_1),\Re(z_2)>0$$where the real part condition ensures that the integral converges.
- $B(z_1,z_2)=\frac{\Gamma(z_1)\Gamma(z_2)}{\Gamma(z_1+z_2)}$.
	- **Proof**: We make use of change of variable. Consider $$\Gamma(z_1)\Gamma(z_2)=\int_0^\infty\int_0^\infty e^{-u-v}u^{z_1-1}u^{z_2-1}dudv$$Now make the substitution $u=st,v=s(1-t)$, then $s\in[0,\infty],t\in[0,1]$, thus $$\begin{align}\Gamma(z_1)\Gamma(z_2)&=\int_0^\infty ds\int_0^1e^{-s}(st)^{z_1-1}(s(1-t))^{z_2-1}sdt\\&=\int_0^\infty e^{-s}s^{z_1+z_2-1}ds\cdot\int_0^1t^{z_1-1}(1-t)^{z_2-1}dt\\&=\Gamma(z_1+z_2)\cdot B(z_1,z_2)\end{align}$$From this we know that $B(z_1,z_2)=B(z_2,z_1)$ (which is also obvious from the definition). Note that another way of substitution is $u=r\sin\theta,v=r\cos\theta$ and notice that $B(z_1,z_2)$ has its trigonometric function expression.
- **Other expressions**
	- Using $t=\cos^2\varphi$ we have $$B(z_1,z_2)=2\int_0^{\pi/2}\cos^{2z_1-1}\varphi\sin^{2z_2-1}\varphi d\varphi$$
	- Using $t=\frac{u}{1+u}$ we have $$B(z_1,z_2)=\int_0^1\frac{u^{z_1-1}+u^{z_2-1}}{(1+u)^{z_1+z_2}}du$$
- **Multivariate beta function** can be defined as $$B(\alpha_1,\alpha_2,\cdots,\alpha_n)=\frac{\Gamma(\alpha_1)\Gamma(\alpha_2)\cdots\Gamma(\alpha_n)}{\Gamma(\alpha_1+\cdots+\alpha_n)}$$which is used for defining the Dirichlet distribution.
- **Application**
	- Note that by change of variable we get $$\int_0^\infty\frac{1}{t^\alpha+1}=\frac{1}{\alpha}\int_0^1s(\frac{1}{s}-1)^{\frac{1}{\alpha}-1}\frac{1}{s^2}ds=\frac{1}{\alpha}B(1-\frac{1}{\alpha},\frac{1}{\alpha})$$