> Given $a_1=-1$ with recurrence relation $$\sum_{k=0}^n\frac{a_{n+1-k}}{k+1}=0,\quad\forall n\ge1$$Show that $a_n\ge0,\forall n\ge2$.
## Matrix method
For convenience we replace index $n$ with $n+1$. The first $n-1$ recurrence relations with $a_1=-1$ forms a linear system $$\begin{bmatrix}1\\\frac{1}{2}&1\\\frac{1}{3}&\frac{1}{2}&1\\\vdots&\vdots&\vdots&\ddots\\\frac{1}{n}&\frac{1}{n-1}&\frac{1}{n-2}&\cdots&1\end{bmatrix}\begin{bmatrix}a_1\\a_2\\a_3\\\vdots\\a_n\end{bmatrix}=\begin{bmatrix}-1\\0\\0\\\vdots\\0\end{bmatrix}$$Hence by Cramer's rule ([[Solving Linear System]]) and [[Determinant]] we have $$a_n=(-1)^n\begin{vmatrix}\frac{1}{2}&1\\\frac{1}{3}&\frac{1}{2}&1\\\vdots&\vdots&\ddots&\ddots\\\vdots&\vdots&\cdots&\frac{1}{2}&1\\\frac{1}{n}&\frac{1}{n-1}&\cdots&\frac{1}{3}&\frac{1}{2}\end{vmatrix}\coloneqq(-1)^n\det A_n$$The above is a Hessenberg matrix whose determinant does not admit a closed form, hence we need to purely analyze its sign pattern. I suspect that this can be done via LU decomposition ([[Matrix Decomposition]]), or induction via constructing a pairing matrix series by adding some new elements, but I fail to find one proof so far.
## Generating function method
Notice that the recurrence relation takes the form of [[Convolution]]. Denote $$f(x)=\sum_{n\in\mathbb N}a_nx^n,\quad g(x)=\sum_{n\in\mathbb N}\frac{x^n}{n+1}=-\frac{\ln(1-x)}{x}$$Then the recurrence relation is implies $f(x)g(x)=-1$, hence $$f(x)=\frac{x}{\ln(1-x)}$$By [[Cauchy Integral]] formula we have that $$a_n=\Res\left(\frac{1}{z^n\ln(1-z)},0\right)$$Utilizing Jordan' lemma ([[Contour Integral]]) we can show that $a_n\ge0$.
## Other info
This is a problem from IMO short list, and the original solution requires quite a lot "attention". I don't personally appreciate that solution much.