**Hermite interpolation** generalizes Lagrange interpolation ([[Polynomial Interpolation]]) by allowing for constraints on the derivatives of the interpolation function, and the basic ideas are the same: notice that in general we have $$\left.\frac{d^m}{dx^m}x^n\right|_0=n!\delta_n^{m}$$hence by general Leibniz rule ([[Differential Calculus on Euclidean Space]]) we have $$\frac{d^m}{dx^m}\left(x^nf(x)\right)=\sum_{k=0}^m\binom{m}{k}n!\delta_n^k f^{(m-k)}(x)=\begin{cases}0,&m<n\\\frac{m!}{(m-n)!}f^{(m-n)}(x),&m\ge n\end{cases}$$This allows us to construct functions satisfying a set of derivative conditions in Newton fashion.
**Uniqueness**: given $\sum(m_i+1)$ data points $(x_i,y_i^{(j)})_{1\le i\le n,0\le j\le m_i}$ consider the congruence system $$H(x)\equiv\sum_{j=0}^{m_i}\frac{y_i^{(j)}}{j!}(x-x_i)^j\mod(x-x_i)^{m_i+1},\quad\forall 1\le i\le n$$by CRT ([[Ideal]]) the solution with $\deg H(x)\le\sum(m_i+1)$ is unique.
- **Lagrange-fashion calculation**: first define a set of basis polynomial $h_{ij}(x)$ satisfying $$h_{ij}^{(t)}(b_s)=\delta_{is}\delta_{jt},\quad\forall1\le i,s\le n,0\le j,t\le m_i$$then it suffices to put all the coefficients into the linear combination to get the interpolation polynomial. Note that we use $i,j$ for indexing $h$, and $s,t$ for indexing $(x_s,y_s^{(t)})$.
- **Newton-fashioned calculation**: we mimic the calculation of Newton interpolation, and make use of the replacement (similar to the one in [[Umbral Calculus]]) $f[x,x,\cdots,x]=\frac{f^{(k)}(x)}{k!}$ (there are $k+1\ x$'s). View the higher-order derivatives as repeated data points, and fill in the divided difference table with the corresponding data would allow us to compute the result.
- **General formula**: the general formula for Hermite interpolation is $$H(x)=\sum_{i=1}^n\sum_{j=0}^{m_i-1}\sum_{k=0}^{m_i-j-1}f^{(j)}(x_i)\frac{1}{j!k!}\left(\frac{(x-x_i)^{m_i}}{\Omega(x)}\right)^{(k)}_{x=x_i}\frac{\Omega(x)}{(x-x_i)^{m_i-j-k}}$$where $\Omega(x)=\prod_i(x-x_i)^{m_i}$. From this we could infer the form of $h_{ij}(x)$.
- **Error**: let $M=\sum(m_i+1)$, then the error is given by $$f(x)-H(x)=\frac{f^{(M)}(c)}{M!}\prod_i(x-x_i)^{m_i},\quad c\in[x_1,x_n]$$
- **Application**: the critical property of Hermite interpolation, that value of derivates up to some order is known for some points, can be utilized to analyze behavior of some operators. 
	- Denote $V$ the linear space of polynomials with degree less than $n$. Given two monic polynomials $\deg f=\deg g=n$, and define $T_1,T_2\in\mathcal B(V)$ by $$T_1(v)\equiv fv\bmod g,\quad T_2(v)\equiv gv\bmod f$$We're interested in $|T_1|,|T_2|$. To calculate this we consider $g(x)=\prod(x-b_s)^{q_s}$ and define the Hermite basis $h_{ij}$ with data points $(b_s,\delta_{is}\delta_{jt})$. Since $h_{ij}$ forms a basis for $V$, we only need to consider the matrix of $T_1$ under $\set{h_{ij}}$. Take $h_{1,0}$ for example, we have $$\begin{align}h_{1,0}(x)f(x)&=u(x)g(x)+r(x)\\ r(b_1)&=h_{1,0}(b_1)f(b_1)=f(b_1)\\ r'(b_1)&=h_{1,0}(b_1)f'(b_1)=f'(b_1)\\ &\ \ \vdots\\ r^{(q_1-1)}(b_1)&=h_{1,0}f^{(q_1-1)}(b_1)=f^{(q_1-1)}(b_1)\end{align}$$since $(x-b_1)^{q_1}\mid g(x)$. Plug in other $b_s$ would always yield $0$, thus $$T_1:h_{1,0}\mapsto \sum_{t=0}^{q_1-1}f^{(j)}(b_1)h_{1t}(x)$$Similarly, for any other $j$ we work out the corresponding expression, given by $$T_1:h_{1,j}\mapsto\sum_{t=j}^{q_1-1}C_t^jf^{(t-j)}(b_1)h_{1t}$$where the Leibniz formula is used. Till now we've found that the under basis $h_{1j}$ the $T_1$ has a lower triangular matrix representation, and this applies to any $h_{sj}$ too. Finally we'd find that the answer is $$|T_1|=\prod_{(x-b_s)^{q_s}\|g(x)}f(b_s)^{q_s},\quad |T_2|=\prod_{(x-a_s)^{p_s}\|f(x)}g(a_s)^{p_s}$$In this solution the function of Hermite basis can be summarized as **indexing** or **masking**.
## Spline interpolation
Instead of one single polynomial, we may try to approximate the original function $f$ on multiple sub-intervals. One of the most commonly used method is to approximate each $f(x),x\in[x_{i-1},x_i]$ with a polynomial. To ensure $S(x)$ is smooth we'd like that our polynomial satisfies $$\begin{cases}S_-(x_{i})=S_+(x_i)=y_i\\ S_-'(x_i)=S_+(x_i)\\ S_-''(x_i)=S_+(x_i)\end{cases},\quad 1\le i\le n-1$$This is possible only when using polynomials with degree $3$ or higher. The classical approach is to use exactly those with degree $3$, which we call **cubic splines**. Since the above contains only $4n-2$ conditions, while there are $4n$ coefficients in total, we'd add $2$ more conditions to ensure uniqueness. We'd usually choose:
- **Natural cubic spline**: $S''(x_0)=S''(x_n)=0$.
- **Clamped cubic spline**: $S'(x_0)=f'(x_0),S'(x_n)=f'(x_n)$.
- **Not-a-knot spline**: $S'''_-(x_1)=S'''_+(x_1),S'''_-(x_{n-1})=S'''_+(x_{n-1})$.
Another kind of spline interpolation can be found in [[Curve Gallery#BÃ©zier spline]], which can be seen as a generalization of cubic spline, in the sense that the parameter takes a cubic form.
- **Calculation**: denote $S''(x_i)=M_i$. Since $S(x)$ is cubic on each interval, then $S''$ would be linear, thus $S''(x)$ can be given, and by integration we could work out the overall expression of $S(x)$ on each $[x_{i-1},x_i]$.
